Started subtyping

theories/PtsSignature.v
@@ -8,6 +8,9 @@ Record PtsSig : Type :=
       Ax : St -> St -> Prop;
       Ru : St -> St -> St -> Set;
       Ru_nat : St -> Set;
+      (** Subtyping *)
+      Ru_sub : St -> St -> Prop;
+      Ru_sub_backwards_ax : forall s1 s2, Ru_sub s1 s2 -> forall s3, Ax s2 s3 -> Ax s1 s3;
     }.
 
 Record PredicativeSig (P : PtsSig) : Type :=
@@ -17,12 +20,14 @@ Record PredicativeSig (P : PtsSig) : Type :=
       wf_rel : well_founded pred_rel;
       ord_ax : forall {s1 s2 : P}, Ax P s1 s2 -> pred_rel s1 s2;
       ord_ru : forall {s1 s2 s3 : P}, Ru P s1 s2 s3 -> (pred_rel s1 s3 \/ s1 = s3) /\ (pred_rel s2 s3 \/ s2 = s3);
+      resp_by_sub : forall {s1 s2 : P}, Ru_sub P s1 s2 -> pred_rel s1 s2;
     }.
 Arguments pred_rel {_}.
 Arguments ord_rel {_}.
 Arguments wf_rel {_}.
 Arguments ord_ax {_} _ {_ _}.
 Arguments ord_ru {_} _ {_ _ _}.
+Arguments resp_by_sub {_} _ {_ _}.
 
 Section OrderProperties.
   Context {P : PtsSig} (pred_P : PredicativeSig P).
@@ -64,166 +69,166 @@ End OrderProperties.
 Definition FullSig (P : PtsSig) : Type := forall s, exists s', Ax P s s'.
 
 
-Section SignatureExtension.
-  Context (P : PtsSig) (pred_P : PredicativeSig P).
+(* Section SignatureExtension. *)
+(*   Context (P : PtsSig) (pred_P : PredicativeSig P). *)
 
-  (** Defining a new signature *)
-  Inductive eSt : Set :=
-  | st_P : St P -> eSt
-  | st_ext : nat -> eSt.
+(*   (** Defining a new signature *) *)
+(*   Inductive eSt : Set := *)
+(*   | st_P : St P -> eSt *)
+(*   | st_ext : nat -> eSt. *)
 
-  Inductive eAx : eSt -> eSt -> Prop :=
-  | ax_P : forall {s1 s2 : St P}, Ax P s1 s2 -> eAx (st_P s1) (st_P s2)
-  | ax_ext : forall {n : nat}, eAx (st_ext n) (st_ext (S n))
-  | ax_cross : forall {s : St P}, eAx (st_P s) (st_ext 0).
+(*   Inductive eAx : eSt -> eSt -> Prop := *)
+(*   | ax_P : forall {s1 s2 : St P}, Ax P s1 s2 -> eAx (st_P s1) (st_P s2) *)
+(*   | ax_ext : forall {n : nat}, eAx (st_ext n) (st_ext (S n)) *)
+(*   | ax_cross : forall {s : St P}, eAx (st_P s) (st_ext 0). *)
 
-  Inductive eRu : eSt -> eSt -> eSt -> Set :=
-  | ru_P : forall {s1 s2 s3 : St P}, Ru P s1 s2 s3 -> eRu (st_P s1) (st_P s2) (st_P s3).
+(*   Inductive eRu : eSt -> eSt -> eSt -> Set := *)
+(*   | ru_P : forall {s1 s2 s3 : St P}, Ru P s1 s2 s3 -> eRu (st_P s1) (st_P s2) (st_P s3). *)
 
-  Inductive eRu_nat : eSt -> Set :=
-  | runat_P : forall {s : St P}, Ru_nat P s -> eRu_nat (st_P s).
+(*   Inductive eRu_nat : eSt -> Set := *)
+(*   | runat_P : forall {s : St P}, Ru_nat P s -> eRu_nat (st_P s). *)
 
-  Definition eP : PtsSig := mkPtsSig eSt eAx eRu eRu_nat.
-
-
-  (** Proof that the extended signature is still predicative *)
-  Inductive epred_rel : relation eP :=
-  | pr_P : forall {s1 s2 : St P}, pred_rel pred_P s1 s2 -> epred_rel (st_P s1) (st_P s2)
-  | pr_ext : forall {i j : nat}, i < j -> epred_rel (st_ext i) (st_ext j)
-  | pr_cross : forall {s : St P} {i : nat}, epred_rel (st_P s) (st_ext i).
+(*   Definition eP : PtsSig := mkPtsSig eSt eAx eRu eRu_nat. *)
 
 
-  Lemma eord_rel : StrictOrder epred_rel.
-  Proof using Type.
-    assert (StrictOrder (pred_rel pred_P)) by (eapply ord_rel).
-    destruct H.
-    split.
-    - intros x Hx.
-      inversion_clear Hx.
-      + eapply StrictOrder_Irreflexive; eauto.
-      + unfold lt in H.
-        induction i.
-        * inversion H.
-        * eapply IHi.
-          eapply le_S_n; assumption.
-    - intros x y z Hxy.
-      inversion_clear Hxy; intros Hyz.
-      + inversion_clear Hyz.
-        * assert (pred_rel pred_P s1 s3) by (eapply StrictOrder_Transitive; eauto).
-          econstructor; auto.
-        * econstructor; auto.
-      + inversion_clear Hyz.
-        assert (i < j0) by (etransitivity; eauto).
-        econstructor; auto.
-      + inversion_clear Hyz.
-        econstructor; auto.
-  Qed.
-
-  Lemma wf_acc_orig : forall (s : P), Acc (pred_rel pred_P) s -> Acc epred_rel (st_P s).
-  Proof using Type.
-    intros.
-    induction H.
-    constructor.
-    intros.
-    assert (exists s' : P, y = (st_P s') /\ pred_rel pred_P s' x).
-    {
-      inversion H1; subst.
-      exists s1; split; auto.
-    }
-    destruct H2 as [s' []].
-    rewrite H2.
-    apply H0.
-    assumption.
-  Qed.
-
-  Lemma wf_acc_nat : forall (i : nat), Acc lt i -> Acc epred_rel (st_ext i).
-  Proof using Type.
-    intros.
-    induction H.
-    constructor.
-    intros.
-    inversion H1; subst.
-    - apply H0; auto.
-    - apply wf_acc_orig.
-      apply (wf_rel pred_P).
-  Qed.
-
-  Lemma wf_acc_lt : forall (i : nat), Acc lt i.
-  Proof using Type.
-    intros i.
-    induction i;
-      constructor; intros.
-    - unfold lt in H.
-      inversion H.
-    - inversion H; auto.
-      destruct IHi; auto.
-  Qed.
-
-  Lemma epred_rel_wf : well_founded epred_rel.
-  Proof using Type.
-    assert (Hwf : well_founded (pred_rel pred_P)) by (apply wf_rel).
-    intros a.
-    constructor.
-    intros b H.
-    inversion_clear H.
-    - apply wf_acc_orig.
-      apply Hwf.
-    - apply wf_acc_nat.
-      apply wf_acc_lt.
-    - apply wf_acc_orig.
-      apply Hwf.
-  Qed.
-
-  Lemma eord_ax : forall (s1 s2 : eP), Ax eP s1 s2 -> epred_rel s1 s2.
-  Proof using Type.
-    intros.
-    inversion_clear H; econstructor; auto.
-    eapply ord_ax; assumption.
-  Qed.
-
-  Lemma eord_ru : forall (s1 s2 s3 : eP), Ru eP s1 s2 s3 -> (epred_rel s1 s3 \/ s1 = s3) /\ (epred_rel s2 s3 \/ s2 = s3).
-  Proof using Type.
-    intros.
-    inversion H; subst.
-    assert (((pred_rel pred_P s0 s5) \/ (s0 = s5)) /\ ((pred_rel pred_P s4 s5) \/ (s4 =s5))) by (apply ord_ru; auto).
-    destruct H1.
-    split.
-    - destruct H1.
-      + left.
-        econstructor; auto.
-      + right.
-        subst; reflexivity.
-    - destruct H2.
-      + left.
-        econstructor; auto.
-      + right.
-        subst; reflexivity.
-  Qed.
+(*   (** Proof that the extended signature is still predicative *) *)
+(*   Inductive epred_rel : relation eP := *)
+(*   | pr_P : forall {s1 s2 : St P}, pred_rel pred_P s1 s2 -> epred_rel (st_P s1) (st_P s2) *)
+(*   | pr_ext : forall {i j : nat}, i < j -> epred_rel (st_ext i) (st_ext j) *)
+(*   | pr_cross : forall {s : St P} {i : nat}, epred_rel (st_P s) (st_ext i). *)
 
 
-  Definition epred_P : PredicativeSig eP :=
-    mkPredicativeSig eP epred_rel eord_rel epred_rel_wf eord_ax eord_ru.
+(*   Lemma eord_rel : StrictOrder epred_rel. *)
+(*   Proof using Type. *)
+(*     assert (StrictOrder (pred_rel pred_P)) by (eapply ord_rel). *)
+(*     destruct H. *)
+(*     split. *)
+(*     - intros x Hx. *)
+(*       inversion_clear Hx. *)
+(*       + eapply StrictOrder_Irreflexive; eauto. *)
+(*       + unfold lt in H. *)
+(*         induction i. *)
+(*         * inversion H. *)
+(*         * eapply IHi. *)
+(*           eapply le_S_n; assumption. *)
+(*     - intros x y z Hxy. *)
+(*       inversion_clear Hxy; intros Hyz. *)
+(*       + inversion_clear Hyz. *)
+(*         * assert (pred_rel pred_P s1 s3) by (eapply StrictOrder_Transitive; eauto). *)
+(*           econstructor; auto. *)
+(*         * econstructor; auto. *)
+(*       + inversion_clear Hyz. *)
+(*         assert (i < j0) by (etransitivity; eauto). *)
+(*         econstructor; auto. *)
+(*       + inversion_clear Hyz. *)
+(*         econstructor; auto. *)
+(*   Qed. *)
 
-  (** Proof that the extended signature is full *)
-  Lemma full_eP : FullSig eP.
-  Proof using Type.
-    intros s.
-    destruct s.
-    - exists (st_ext 0).
-      econstructor.
+(*   Lemma wf_acc_orig : forall (s : P), Acc (pred_rel pred_P) s -> Acc epred_rel (st_P s). *)
+(*   Proof using Type. *)
+(*     intros. *)
+(*     induction H. *)
+(*     constructor. *)
+(*     intros. *)
+(*     assert (exists s' : P, y = (st_P s') /\ pred_rel pred_P s' x). *)
+(*     { *)
+(*       inversion H1; subst. *)
+(*       exists s1; split; auto. *)
+(*     } *)
+(*     destruct H2 as [s' []]. *)
+(*     rewrite H2. *)
+(*     apply H0. *)
+(*     assumption. *)
+(*   Qed. *)
 
-    - exists (st_ext (S n)).
-      econstructor.
-  Qed.
-End SignatureExtension.
+(*   Lemma wf_acc_nat : forall (i : nat), Acc lt i -> Acc epred_rel (st_ext i). *)
+(*   Proof using Type. *)
+(*     intros. *)
+(*     induction H. *)
+(*     constructor. *)
+(*     intros. *)
+(*     inversion H1; subst. *)
+(*     - apply H0; auto. *)
+(*     - apply wf_acc_orig. *)
+(*       apply (wf_rel pred_P). *)
+(*   Qed. *)
 
-Arguments st_P {P} s.
-Arguments st_ext {P} i.
-Arguments ax_P {P} {s1} {s2} ax.
-Arguments ax_ext {P} {n}.
-Arguments ax_cross {P} {s}.
-Arguments ru_P {P} {s1} {s2} {s3} ru.
+(*   Lemma wf_acc_lt : forall (i : nat), Acc lt i. *)
+(*   Proof using Type. *)
+(*     intros i. *)
+(*     induction i; *)
+(*       constructor; intros. *)
+(*     - unfold lt in H. *)
+(*       inversion H. *)
+(*     - inversion H; auto. *)
+(*       destruct IHi; auto. *)
+(*   Qed. *)
 
-Arguments pr_P {P} {pred_P} {s1} {s2} pr.
-Arguments pr_ext {P} {pred_P} {i} {j} lt.
-Arguments pr_cross {P} {pred_P} {s} {i}.
+(*   Lemma epred_rel_wf : well_founded epred_rel. *)
+(*   Proof using Type. *)
+(*     assert (Hwf : well_founded (pred_rel pred_P)) by (apply wf_rel). *)
+(*     intros a. *)
+(*     constructor. *)
+(*     intros b H. *)
+(*     inversion_clear H. *)
+(*     - apply wf_acc_orig. *)
+(*       apply Hwf. *)
+(*     - apply wf_acc_nat. *)
+(*       apply wf_acc_lt. *)
+(*     - apply wf_acc_orig. *)
+(*       apply Hwf. *)
+(*   Qed. *)
+
+(*   Lemma eord_ax : forall (s1 s2 : eP), Ax eP s1 s2 -> epred_rel s1 s2. *)
+(*   Proof using Type. *)
+(*     intros. *)
+(*     inversion_clear H; econstructor; auto. *)
+(*     eapply ord_ax; assumption. *)
+(*   Qed. *)
+
+(*   Lemma eord_ru : forall (s1 s2 s3 : eP), Ru eP s1 s2 s3 -> (epred_rel s1 s3 \/ s1 = s3) /\ (epred_rel s2 s3 \/ s2 = s3). *)
+(*   Proof using Type. *)
+(*     intros. *)
+(*     inversion H; subst. *)
+(*     assert (((pred_rel pred_P s0 s5) \/ (s0 = s5)) /\ ((pred_rel pred_P s4 s5) \/ (s4 =s5))) by (apply ord_ru; auto). *)
+(*     destruct H1. *)
+(*     split. *)
+(*     - destruct H1. *)
+(*       + left. *)
+(*         econstructor; auto. *)
+(*       + right. *)
+(*         subst; reflexivity. *)
+(*     - destruct H2. *)
+(*       + left. *)
+(*         econstructor; auto. *)
+(*       + right. *)
+(*         subst; reflexivity. *)
+(*   Qed. *)
+
+
+(*   Definition epred_P : PredicativeSig eP := *)
+(*     mkPredicativeSig eP epred_rel eord_rel epred_rel_wf eord_ax eord_ru. *)
+
+(*   (** Proof that the extended signature is full *) *)
+(*   Lemma full_eP : FullSig eP. *)
+(*   Proof using Type. *)
+(*     intros s. *)
+(*     destruct s. *)
+(*     - exists (st_ext 0). *)
+(*       econstructor. *)
+
+(*     - exists (st_ext (S n)). *)
+(*       econstructor. *)
+(*   Qed. *)
+(* End SignatureExtension. *)
+
+(* Arguments st_P {P} s. *)
+(* Arguments st_ext {P} i. *)
+(* Arguments ax_P {P} {s1} {s2} ax. *)
+(* Arguments ax_ext {P} {n}. *)
+(* Arguments ax_cross {P} {s}. *)
+(* Arguments ru_P {P} {s1} {s2} {s3} ru. *)
+
+(* Arguments pr_P {P} {pred_P} {s1} {s2} pr. *)
+(* Arguments pr_ext {P} {pred_P} {i} {j} lt. *)
+(* Arguments pr_cross {P} {pred_P} {s} {i}. *)
